Improve compiler for CPP submission.

compiler/lvcc.ml
@@ -14,18 +14,16 @@ let main () =
   let _ = register_name "n" in
   let infile = ref "" in
   let outfile = ref "a.s" in
-  let toILF = ref false in
-  let optimize = ref false in
+  let do_addParams = ref false in
   let toILI = ref false in
-  let set_toILF b = toILF := b in
-  let set_optimize b = optimize := b in
+  let set_addParams b = do_addParams := b in
   let set_toILI b = toILI := b in
   let set_infile s = infile:=s in
   let speclist = [
-    ("-o",Arg.Set_string outfile, "<file> Place the output into <file>");
-    ("-1", Arg.Bool set_toILF, "<bool> Enable IL/I to IL/F phase (default is false)");
-    ("-2", Arg.Bool set_optimize, "<bool> Enable optimization (default is false)");
-    ("-3", Arg.Bool set_toILI, "<bool> Enable IL/F to IL/I phase (default is false)")
+    ("-o", Arg.Set_string outfile, "<file> Place the output into <file>");
+    (*    ("-1", Arg.Bool set_DCE, "<bool> DCE on IL/I input (default is true)"); *)
+    ("-c", Arg.Bool set_addParams, "<bool> Translate to IL/F (default is false)");
+    (*    ("-3", Arg.Bool set_toILI, "<bool> Enable IL/F to IL/I phase (default is false)") *)
   ] in
   (*let print_string a s = Printf.eprintf "%s" (camlstring_of_coqstring s); a in
   let toString_nstmt s = explode (print_nstmt !ids 0 s) in
@@ -33,48 +31,52 @@ let main () =
   let toString_ann s p a = explode (print_ann (fun s -> implode (p s)) 0 a) in
   let toString_set s = explode (print_set !ids s) in
   let toString_list s = explode (print_list (fun x -> print_var !ids x) "," s) in *)
-    Arg.parse speclist set_infile ("usage: lvc [options]");
+    Arg.parse speclist set_infile ("usage: lvcc [options]");
     try
-      if (not !toILF) && (not !optimize) && (not !toILI) then
-	raise (Compiler_error "No translation phase selected, try --help.")
-      else
       (* Printf.printf "Compiling"; *)
       let file_chan = open_in !infile in
       let lexbuf = Lexing.from_channel  file_chan in
       let ilin = Parser.program Lexer.token lexbuf in
-      let _ =  Printf.printf "Input:\n%s\n\n" (print_nstmt !ids 0 ilin) in
+      let _ =  Printf.printf "Input (functions named):\n%s\n\n" (print_nstmt !ids 0 ilin) in
       let ili = (match Compiler.toDeBruijn ilin with
 		 | Success ili -> ili
 		 | Error e -> raise (Compiler_error "Converting to de bruijn failed (did you define all functions?)"))
 		 in
+      let (s_dce, lv_dce) =
+	(let x = Compiler.coq_DCVE ili in
+	 Printf.printf "after DCE (functions de-bruijn):\n%s\n\n" (print_stmt !ids 0 (fst x));
+	 x)
+      in
       let ilf =
-	if !toILF then
-	  let comp = Compiler.toILF ili in
-	  Printf.printf "to ILF:\n%s\n\n" (print_stmt !ids 0 comp);
-	  comp
+	if !do_addParams then
+	  let x = Compiler.addParams s_dce lv_dce in
+	  Printf.printf "as IL/F program (functions de-bruijn):\n%s\n\n" (print_stmt !ids 0 x);
+	  x
 	else
-	  ili in
+	  (Printf.printf "to IL/F program translation disabled, enable with argument -c true\n";
+	  s_dce)
+(*      in
       let sopt =
-(*	if !optimize then
+	if !optimize then
 	  (match Lvc.optimize generic_first ilf with
 	   | Lvc.Success sopt ->
 	      Printf.printf "\noptimized compilate:\n%s\n\n" (print_stmt !ids 0 sopt);
 	      sopt
 	   | Lvc.Error e -> raise (Compiler_error (implode e))
 	   )
-	else *)
+	else
 	ilf
       in
       let res =
-	(* if !toILI then
+	 if !toILI then
           (match Compiler.fromILF parallel_move generic_first sopt with
 	   | Lvc.Success ili ->
 	      Printf.printf "\nto IL/I compilate (functions are de-bruijn now):\n%s\n\n" (print_stmt !ids 0 ili);
 	      ili
 	   | Lvc.Error e -> raise (Compiler_error (implode e))
 	  )
-	else *)
-	sopt
+	else
+	sopt*)
       in ()
     with Parsing.Parse_error -> Printf.eprintf "A parsing error occured \n"
       | Sys_error s-> Printf.eprintf "%s\n" s
